

For latest updates of this note, visit <https://xiaoshuo-lin.github.io/001707E>.

Problem 1 (Maps to \mathbb{S}^n)

- (1) Prove that any non-surjective continuous map $f: X \rightarrow \mathbb{S}^n$ is null-homotopic.
- (2) Let $f, g: X \rightarrow \mathbb{S}^n$ be continuous maps. Suppose they are never antipodal, i.e., $g(x) \neq -f(x)$ holds for all x . Prove that f is homotopic to g .
- (3) Prove that $f \in C(X, Y)$ is null-homotopic if and only if f has a continuous extension $F \in C(C(X), Y)$, where $C(X)$ denotes the cone over X .
- (4) Let \mathbb{D}^{n+1} be the closed unit ball in \mathbb{R}^{n+1} . Prove that there exists a retraction $f \in C(\mathbb{D}^{n+1}, \mathbb{S}^n)$ if and only if $\text{Id}_{\mathbb{S}^n}$ is null-homotopic.

Proof (1) Without loss of generality, assume $N = (0, \dots, 0, 1) \notin f(X)$ and consider the stereographic projection

$$\sigma: \mathbb{S}^n \setminus \{N\} \rightarrow \mathbb{R}^n, \quad (x_1, \dots, x_{n+1}) \mapsto \frac{1}{1 - x_{n+1}}(x_1, \dots, x_n).$$

It is a homeomorphism with inverse

$$\sigma^{-1}: \mathbb{R}^n \rightarrow \mathbb{S}^n \setminus \{N\}, \quad (u_1, \dots, u_n) \mapsto \frac{1}{|u|^2 + 1}(2u_1, \dots, 2u_n, |u|^2 - 1).$$

Then $F(t, x) = \sigma^{-1}((1 - t)\sigma(f(x)))$ is a homotopy from f to the constant map $x \mapsto (0, \dots, 0, -1)$.

- (2) Since $f(x)$ and $g(x)$ are never antipodal, their convex combination $(1 - t)f(x) + tg(x)$ is never zero. Thus the map $H(t, x) = \frac{(1 - t)f(x) + tg(x)}{\|(1 - t)f(x) + tg(x)\|}$ is well-defined and is a homotopy from f to g .

- (3) Let us specify $C(X) = ([0, 1] \times X)/(\{1\} \times X)$.

(\Rightarrow) Let $H: [0, 1] \times X \rightarrow Y$ be a homotopy from f to a constant map c_{y_0} , for some $y_0 \in Y$. Then $H(0, x) = f(x)$ and $H(1, x) = y_0$ for all $x \in X$. Since H is constant on the subspace $\{1\} \times X$, it induces a continuous map $\tilde{H}: C(X) \rightarrow Y$ which agrees with f on $\{0\} \times X$. Thus \tilde{H} is an extension of f to $C(X)$.

(\Leftarrow) Suppose $F \in C(C(X), Y)$ is an extension of f . Then the map

$$H: [0, 1] \times X \rightarrow Y \quad (t, x) \mapsto F([(t, x)])$$

is a homotopy from f to the constant map $x \mapsto F([(1, x)])$.

- (4) (\Rightarrow) Suppose $f \in C(\mathbb{D}^{n+1}, \mathbb{S}^n)$ is a retraction. Then the map

$$F: [0, 1] \times \mathbb{S}^n \rightarrow \mathbb{S}^n, \quad (t, x) \mapsto f((1 - t)x)$$

is a homotopy from $\text{Id}_{\mathbb{S}^n}$ to the constant map $x \mapsto f(0) \in \mathbb{S}^n$.

(\Leftarrow) Suppose $F: [0, 1] \times \mathbb{S}^n \rightarrow \mathbb{S}^n$ is a homotopy from $\text{Id}_{\mathbb{S}^n}$ to a constant map. Fix any point $p_0 \in \mathbb{S}^n$. Then the map $f \in C(\mathbb{D}^{n+1}, \mathbb{S}^n)$, defined by

$$f(x) = \begin{cases} F(1, p_0), & x = 0, \\ F\left(1 - \|x\|, \frac{x}{\|x\|}\right), & x \neq 0, \end{cases}$$

is a retraction. It is continuous since $F(1, x)$ is constant for all $x \in \mathbb{S}^n$. \square

Problem 2 Suppose $f: \mathbb{S}^1 \rightarrow \mathbb{S}^1$ is a map which is not homotopic to the identity. Show that $f(x) = -x$ for some $x \in \mathbb{S}^1$.

Proof This is an immediate corollary of Problem 1 (2), by taking $g = \text{Id}_{\mathbb{S}^1}$. \square

Problem 3 Show that any two continuous maps $f, g: X \rightarrow C(Y)$ are homotopic, where $C(Y)$ denotes the cone over Y .

Proof It suffices to show that any continuous map $f: X \rightarrow C(Y)$ is null-homotopic, and by Problem 1 (3), this is equivalent to showing that f has a continuous extension $F \in C(C(X), C(Y))$.

Since $C(Y) = ([0, 1] \times Y)/(\{1\} \times Y)$, we may write $f(x) = [(t(x), y(x))]$ for some continuous maps $t: X \rightarrow [0, 1]$ and $y: X \rightarrow Y$. Now define the continuous map

$$F: C(X) = ([0, 1] \times X)/(\{1\} \times X) \rightarrow C(Y), \quad [(s, x)] \mapsto [((1-s)t(x) + s, y(x))].$$

F is well-defined We have $F([(1, x)]) = [1, y(x)]$ which is the cone point of $C(Y)$, for all $x \in X$.

$F|_{\{0\} \times X} = f$ We have $F([(0, x)]) = [(t(x), y(x))] = f(x)$ for all $x \in X$.

Thus F is a continuous extension of f to $C(X)$, and the proof is complete. \square

Problem 4 Let X be a path-connected space. Recall that any path $\lambda: [0, 1] \rightarrow X$ with $\lambda(0) = x_0$ and $\lambda(1) = x_1$ induces a group isomorphism

$$\Gamma_\lambda: \pi_1(X, x_0) \rightarrow \pi_1(X, x_1), \quad \langle \gamma \rangle \mapsto \langle \lambda^{-1} * \gamma * \lambda \rangle.$$

Prove that $\pi_1(X, x_0)$ is abelian if and only if for any two paths λ_1, λ_2 from x_0 to x_1 , we have $\Gamma_{\lambda_1} = \Gamma_{\lambda_2}$.

Proof (\Rightarrow) If there exist two paths λ_1, λ_2 from x_0 to x_1 such that $\Gamma_{\lambda_1}(\langle \gamma \rangle) \neq \Gamma_{\lambda_2}(\langle \gamma \rangle)$ for some $\langle \gamma \rangle \in \pi_1(X, x_0)$, i.e., $\langle \lambda_1^{-1} * \gamma * \lambda_1 \rangle \neq \langle \lambda_2^{-1} * \gamma * \lambda_2 \rangle$, then

$$\langle \lambda_2 * \lambda_1^{-1} * \gamma \rangle = \langle \lambda_2 \rangle \langle \lambda_1^{-1} * \gamma * \lambda_1 \rangle \langle \lambda_1^{-1} \rangle \neq \langle \lambda_2 \rangle \langle \lambda_2^{-1} * \gamma * \lambda_2 \rangle \langle \lambda_1^{-1} \rangle = \langle \gamma * \lambda_2 * \lambda_1^{-1} \rangle.$$

This shows that the elements $\langle \gamma \rangle$ and $\langle \lambda_2 * \lambda_1^{-1} \rangle$ do not commute, a contradiction.

(\Leftarrow) For any two loops γ_1, γ_2 based at x_0 , by assumption we have $\Gamma_{\gamma_1}(\langle \gamma_2 \rangle) = \Gamma_{\gamma_2}(\langle \gamma_2 \rangle)$, i.e.,

$$\langle \gamma_1^{-1} * \gamma_2 * \gamma_1 \rangle = \langle \gamma_2^{-1} * \gamma_2 * \gamma_2 \rangle = \langle \gamma_2 \rangle.$$

Thus $\langle \gamma_1 \rangle \langle \gamma_2 \rangle = \langle \gamma_1 \rangle \langle \gamma_1^{-1} * \gamma_2 * \gamma_1 \rangle = \langle \gamma_2 \rangle \langle \gamma_1 \rangle$. \square

Problem 5 Suppose X is connected, and $p: \tilde{X} \rightarrow X$ be a covering map. Show that the cardinality of the fiber $p^{-1}(x)$ is the same for all $x \in X$.

Proof Any $x \in X$ has an open neighborhood U_x homeomorphic to an open neighborhood V_α in \tilde{X} with $p(V_\alpha) = U_x$. For any $y \in U_x$, since $p^{-1}(y) \cap V_\alpha$ contains exactly one point, we have $|p^{-1}(y)| = |p^{-1}(x)|$.

Fix $x_0 \in X$ and let $A = \{x \in X : |p^{-1}(x)| = |p^{-1}(x_0)|\}$. Then both A and A^c are open. Since X is connected and $A \neq \emptyset$, we must have $A = X$, i.e., the cardinality of $p^{-1}(x)$ is the same for all $x \in X$. \square

Remark One can compare the above proof with the proof of Theorem 10.14 in the textbook. //

Problem 6 If $p: \tilde{X} \rightarrow X$ and $q: \tilde{Y} \rightarrow Y$ are two covering maps, show that $p \times q: \tilde{X} \times \tilde{Y} \rightarrow X \times Y$ is also a covering map.

Proof Given $(x, y) \in X \times Y$, let U be an open neighborhood of x in X such that $p^{-1}(U)$ is a disjoint union of open sets V_α in \tilde{X} and $p|_{V_\alpha}: V_\alpha \rightarrow U$ is a homeomorphism for each α . Similarly, let U' be an open neighborhood of y in Y such that $q^{-1}(U')$ is a disjoint union of open sets V'_β in \tilde{Y} and $q|_{V'_\beta}: V'_\beta \rightarrow U'$ is a homeomorphism for each β . Then

- ◇ $U \times U'$ is an open neighborhood of (x, y) in $X \times Y$.
- ◇ $(p \times q)^{-1}(U \times U') = p^{-1}(U) \times q^{-1}(U')$ is a disjoint union of open sets $V_\alpha \times V'_\beta$ in $\tilde{X} \times \tilde{Y}$.
- ◇ $(p \times q)|_{V_\alpha \times V'_\beta} = (p|_{V_\alpha}) \times (q|_{V'_\beta})$ is a homeomorphism for all α, β . □

Remark It is then natural to ask whether the product of infinitely many covering maps is still a covering map. The answer is **negative** in general. To see this, one first needs to prove the following formula for the fundamental group of an arbitrary product. For an arbitrary collection of path-connected spaces X_α there is a group isomorphism (try it yourself!)

$$\pi_1\left(\prod_{\alpha} X_{\alpha}\right) \simeq \prod_{\alpha} \pi_1(X_{\alpha}). \quad (\text{P6-1})$$

Now, let $p: \mathbb{R} \rightarrow \mathbb{S}^1$ be the standard covering map. We claim that the infinite product

$$P = \prod_{n=1}^{\infty} p: \prod_{n=1}^{\infty} \mathbb{R} \rightarrow \prod_{n=1}^{\infty} \mathbb{S}^1$$

is **not** a covering map. Indeed, were it a covering map, then some open neighborhood U of $(0, 0, \dots)$ in $\prod_{n=1}^{\infty} \mathbb{R}$ would be mapped by P homeomorphically to some neighborhood V of $(1, 1, \dots)$ in $\prod_{n=1}^{\infty} \mathbb{S}^1$. By shrinking we can assume $U = (-a_1, a_1) \times \dots \times (-a_k, a_k) \times \mathbb{R} \times \mathbb{R} \times \dots$, so that U is contractible, and $P(U)$ has infinitely many \mathbb{S}^1 factors. By (P6-1),

$$\{e\} = \pi_1(U) \simeq \pi_1(P(U)) \simeq \prod_{n=1}^k \pi_1(p(-a_n, a_n)) \times \prod_{n=k+1}^{\infty} \pi_1(\mathbb{S}^1) \neq \{e\},$$

which is a contradiction. //

We say two paths $\gamma_0, \gamma_1: [0, 1] \rightarrow X$ are path-homotopic, denoted as $\gamma_1 \sim_p \gamma_0$, if

- ◇ $\gamma_0(0) = \gamma_1(0) = x_0, \gamma_0(1) = \gamma_1(1) = x_1$, and
- ◇ there exists a continuous map $F: [0, 1] \times [0, 1] \rightarrow X$ such that

$$\begin{aligned} F(0, t) &= \gamma_0(t) & \text{and} & & F(1, t) &= \gamma_1(t), & \forall t \in [0, 1], \\ F(s, 0) &= x_0 & \text{and} & & F(s, 1) &= x_1, & \forall s \in [0, 1]. \end{aligned}$$

Problem 7 (Fundamental group of a topological group) Let (G, \bullet) be a path-connected topological group. We want to prove that $\pi_1(G, e)$ is an abelian group. Let γ_1, γ_2 be two loops in G based at e .

(1) (First proof) Denote by γ_e the constant loop at e . Verify that

$$F(s, t) = (\gamma_1 * \gamma_e)(\max\{0, t - \frac{s}{2}\}) \bullet (\gamma_e * \gamma_2)(\min\{1, t + \frac{s}{2}\})$$

is a path-homotopy between $\gamma_1 * \gamma_2$ and $\gamma_2 * \gamma_1$, where \bullet is the group multiplication.

(2) (Second proof) Construct explicit path-homotopies to verify that

$$\textcircled{1} \quad \gamma_1(t) \bullet \gamma_2(t) \underset{p}{\sim} \gamma_2(t) \bullet \gamma_1(t).$$

$$\textcircled{2} \quad (\gamma_1 * \gamma_2)(t) \underset{p}{\sim} \gamma_1(t) \bullet \gamma_2(t).$$

(3) (Third proof, the Eckmann–Hilton argument)

$\textcircled{1}$ Let S be a set on which there are two “semigroup with unitary” structures, $(S, \circ, 1_\circ)$ and $(S, \bullet, 1_\bullet)$. Moreover, suppose

$$(g \circ h) \bullet (g' \circ h') = (g \bullet g') \circ (h \bullet h'), \quad \forall g, g', h, h' \in S.$$

Prove that $1_\circ = 1_\bullet$, $g \bullet h = g \circ h$, and $g \circ h = h \circ g$.

$\textcircled{2}$ Define $\langle \gamma_1 \rangle_p \bullet \langle \gamma_2 \rangle_p = \langle \gamma_1 \bullet \gamma_2 \rangle_p$. Show that \bullet is well-defined on $\pi_1(G, e)$.

$\textcircled{3}$ Use $\textcircled{1}$ to prove that $\pi_1(G)$ is abelian.

Proof (1) Clearly $F(s, t) \in C([0, 1] \times [0, 1], G)$.

When $s = 0$, we have

$$\begin{aligned} F(0, t) &= (\gamma_1 * \gamma_e)(t) \bullet (\gamma_e * \gamma_2)(t) \\ &= \begin{cases} \gamma_1(2t) \bullet \gamma_e(2t) = \gamma_1(2t), & 0 \leq t \leq \frac{1}{2}, \\ \gamma_e(2t-1) \bullet \gamma_2(2t-1) = \gamma_2(2t-1), & \frac{1}{2} \leq t \leq 1, \end{cases} \\ &= \gamma_1 * \gamma_2(t). \end{aligned} \tag{P7-1}$$

When $s = 1$, we have

$$\begin{aligned} F(1, t) &= (\gamma_1 * \gamma_e)(\max\{0, t - \frac{1}{2}\}) \bullet (\gamma_e * \gamma_2)(\min\{1, t + \frac{1}{2}\}) \\ &= \begin{cases} (\gamma_1 * \gamma_e)(0) \bullet (\gamma_e * \gamma_2)(t + \frac{1}{2}) = \gamma_2(2t), & 0 \leq t \leq \frac{1}{2}, \\ (\gamma_1 * \gamma_e)(t - \frac{1}{2}) \bullet (\gamma_e * \gamma_2)(1) = \gamma_1(2t-1), & \frac{1}{2} \leq t \leq 1, \end{cases} \\ &= \gamma_2 * \gamma_1(t). \end{aligned}$$

(2) $\textcircled{1}$ Consider $F(s, t) = (\gamma_1(ts))^{-1} \bullet \gamma_1(t) \bullet \gamma_2(t) \bullet \gamma_1(ts)$. We have

$$F(0, t) = \gamma_1(t) \bullet \gamma_2(t), \quad F(1, t) = \gamma_2(t) \bullet \gamma_1(t).$$

② Consider $F(s, t) = (\gamma_1 * \gamma_e)(t(1 - \frac{s}{2})) \bullet (\gamma_e * \gamma_2)(t(1 - \frac{s}{2}) + \frac{s}{2})$. We have

$$\begin{aligned} F(0, t) &= (\gamma_1 * \gamma_e)(t) \bullet (\gamma_e * \gamma_2)(t) \stackrel{(P7-1)}{=} \gamma_1 * \gamma_2(t), \\ F(1, t) &= (\gamma_1 * \gamma_e)(\frac{t}{2}) \bullet (\gamma_e * \gamma_2)(\frac{t+1}{2}) = \gamma_1(t) \bullet \gamma_2(t). \end{aligned}$$

(3) ① The units of the two operations coincide:

$$1_\circ = 1_\circ \circ 1_\circ = (1_\bullet \bullet 1_\circ) \circ (1_\circ \bullet 1_\bullet) = (1_\bullet \circ 1_\circ) \bullet (1_\circ \bullet 1_\bullet) = 1_\bullet \bullet 1_\bullet = 1_\bullet.$$

For any $g, h \in S$, we have

$$\begin{aligned} [\overline{g \circ h}] &= (1 \bullet g) \circ (h \bullet 1) = (1 \circ h) \bullet (g \circ 1) = [\overline{h \bullet g}] \\ &= (h \circ 1) \bullet (1 \circ g) = (h \bullet 1) \circ (1 \bullet g) = [\overline{h \circ g}]. \end{aligned}$$

- ② Suppose γ_i ($i = 1, 2, 3, 4$) are loops in G based at e such that $\gamma_1 \underset{p}{\sim} \gamma_2$ and $\gamma_3 \underset{p}{\sim} \gamma_4$. Let F, G be their respective path-homotopies. Then $F \bullet H$ is a path-homotopy between $\gamma_1 \bullet \gamma_3$ and $\gamma_2 \bullet \gamma_4$.
- ③ Now $(\pi_1(G, e), *, \gamma_e)$ and $(\pi_1(G, e), \bullet, \gamma_e)$ are two “semigroup with unitary” structures on $\pi_1(G, e)$. Moreover, for any $\langle \gamma_i \rangle \in \pi_1(G, e)$ ($i = 1, 2, 3, 4$), we have

$$(\langle \gamma_1 \rangle * \langle \gamma_2 \rangle) \bullet (\langle \gamma_3 \rangle * \langle \gamma_4 \rangle) = (\langle \gamma_1 \rangle \bullet \langle \gamma_3 \rangle) * (\langle \gamma_2 \rangle \bullet \langle \gamma_4 \rangle).$$

By ①, $\pi_1(G) \simeq (\pi_1(G, e), *, \gamma_e)$ is abelian. □